Add forward/backward transforming predcate monads

src/QingLong/DijkstraMonad.lean
@@ -1,88 +1,157 @@
 universe u v
 
-def Top {s : Type} : s → Prop := fun _ => True
-
+--
+-- a simple monad along with a proof that the monad returns a specific value
+--
 
 structure BaseMonad (α : Type) where
   (output : α)
 
-inductive MonadResultIs {α : Type} : α → BaseMonad α → Prop where
-| mk : (z : α) → (mz : BaseMonad α) → (mz.output = z) → MonadResultIs z mz
+inductive MonadResultIs {α : Type} : α → Type where
+| mk : (mz : BaseMonad α) → MonadResultIs (mz.output)
 
-def MRret {α : Type} (a : α) := MonadResultIs.mk a (BaseMonad.mk a) rfl
+def MRret {α : Type} (a : α) := MonadResultIs.mk (BaseMonad.mk a)
 
-def MRbind {α : Type} {a b : α} {ma mb : BaseMonad α} : MonadResultIs a ma → (α → MonadResultIs b mb) → MonadResultIs b mb :=
+def MRbind {α : Type} {a b : α} {ma mb : BaseMonad α} : MonadResultIs a → (α → MonadResultIs b) → MonadResultIs b :=
   fun m1 m2 => match m1 with
-               | MonadResultIs.mk z mz zp => m2 z
+               | MonadResultIs.mk mz => m2 (mz.output)
 
-def MRrun {α : Type} {z : α} {mz : BaseMonad α} (d : MonadResultIs z mz) : α :=
+def MRrun {α : Type} {z : α} {mz : BaseMonad α} (d : MonadResultIs z) : α :=
   match d with
-  | MonadResultIs.mk r _ hp => r
+  | MonadResultIs.mk mz => mz.output
 
 
 #check MRret 3
-#check MRrun (MRret 3)
--- here we try to run the monad and enforce a return value that is wrong, should produce and error
+#reduce MRrun (MRret 3)
+#reduce MRrun (MRbind (MRret 2) (fun _ => MRret 3))
+-- here we try to run the monad and enforce a return value (4) that is wrong (actually returns 3).  This should produce and error
 #check @MRrun Nat 4 _ (MRret 3)
 
-inductive Eeek {α : Type} : α → α → Prop where
-| EeekRaf : (z : α) → Eeek z z
 
-def raff {α : Type} {a : α} : Eeek a a:= Eeek.EeekRaf a
+def dPred (α : Type) : Type := α → Prop
 
-#check show Eeek 3 3 by apply raff
+def retEqPred {α : Type} (v : α) : dPred α := fun y => y = v
+def retEqProof {α : Type} (v : α) : retEqPred v v := show v = v by rfl
+
+def bindPred {α β : Type} (p : dPred α) (f : α → dPred β) : dPred β := fun b => ∃ (a:α), p a ∧ f a b
+
+inductive MonadWithPredicate {α : Type} : α → dPred α → Type where
+| mk : (mz : BaseMonad α) → (pf : p mz.output) → MonadWithPredicate (mz.output) p
+
+def retMW {α : Type} {p : dPred α} (v : α) (pf : p v) := MonadWithPredicate.mk (BaseMonad.mk v) pf
+
+-- bind that just uses the predicate of the most recent monad. All monads need to use the same predicate here.
+def bindMW {α : Type} {p : dPred α} {a b : α} {ma mb : BaseMonad α} : MonadWithPredicate a p → (α → MonadWithPredicate b p) → MonadWithPredicate b p :=
+  fun m1 m2 => match m1 with
+               | MonadWithPredicate.mk mz1 pf1 => m2 mz1.output
+
+-- bind that combines (using AND) the predicates of both monads
+def bindMWAnd {α : Type} {p₁ p₂ : dPred α} {a b : α} : MonadWithPredicate a p₁ → (α → MonadWithPredicate b p₂) → MonadWithPredicate b (fun b => ∃x, p₁ x ∧ (p₂ b)) :=
+  fun m1 m2 => match m1 with
+               | MonadWithPredicate.mk mz1 pf1 =>
+                 match (m2 mz1.output) with
+                 | MonadWithPredicate.mk mz2 pf2 =>
+                     MonadWithPredicate.mk mz2 (show ∃ x, p₁ x ∧ p₂ mz2.output from Exists.intro mz1.output (And.intro pf1 pf2))
+
+def runPred {α : Type} {a : α} (p : dPred α) (m : MonadWithPredicate (a : α) p) : p a :=
+  match m with
+  | MonadWithPredicate.mk b pf => pf
+
+
+#check show ∃ x, x=3 from Exists.intro 3 (_:3=3)
+#reduce (retMW 3 _ : MonadWithPredicate 3 (retEqPred 3))
+#reduce (retMW 3 (retEqProof 3) : MonadWithPredicate 3 (retEqPred 3))
+#reduce (runPred (retEqPred 3) (retMW 3 _))
+#reduce (runPred _ (bindMW (retMW 3 (retEqProof 3)) (fun _ => retMW 3 (retEqProof 3))))
+#reduce (runPred _ (bindMWAnd (retMW 3 (retEqProof 3)) (fun _ => retMW 4 (retEqProof 4))))
+
+def runProg := runPred (retEqPred 3) (retMW 3 (retEqProof 3))
+def runProg2 := (runPred _ (bindMWAnd (retMW 3 (retEqProof 3)) (fun (x : Nat) => retMW 4 (retEqProof 4))))
+
+
+#check @runProg2
+#check Exists.intro 3 rfl
+#check (show (∃ x, x = 3) from (Exists.intro 3 rfl))
+#check (show (∀ a, a = 3 → retEqPred 3 3) from (fun a (_:a=3) => _))
+#check Exists.elim (show (∃ x, x = 3) from (Exists.intro 3 rfl)) (show (∀ a, a = 3 → retEqPred 3 3) from (fun a (_:a=3) => _))
+
+
+example (h: ∃ x, retEqPred 3 x ∧ retEqPred 4 4) : retEqPred 3 3 := by
+  let hx : ∀ a, retEqPred 3 a ∧ retEqPred 4 4 → retEqPred 3 3 := show ∀a, retEqPred 3 a ∧ retEqPred 4 4 → retEqPred 3 3 from (fun a x => show _ from rfl)
+  apply Exists.elim h hx
+
+-- forward transforming predicate
+
+def fPred (α : Type) : Type := Prop → α → Prop
+
+def simpleFP {α : Type} (v : α) : fPred α := fun (pre:Prop) (a : α) => pre ∧ a = v
+
+
+inductive MonadFwdPredicate {α : Type} : Prop → α → fPred α → Type where
+| mk : (mz : BaseMonad α) → (pf : ∀ (hpre : pre), p pre mz.output) → MonadFwdPredicate pre (mz.output) p
+
+
+def retFP {α : Type} (v : α) {pre :Prop} : MonadFwdPredicate pre v (@simpleFP α v) :=
+  let bm := BaseMonad.mk v
+  MonadFwdPredicate.mk bm (fun (hpre : pre) => show simpleFP v pre bm.output from (And.intro hpre rfl))
+
+def bindFP {α :Type} {a b : α} {pre1 : Prop} {p₁ p₂ : fPred α} :
+  MonadFwdPredicate pre1 a p₁ → (α → MonadFwdPredicate (p₁ pre1 a) b p₂) → MonadFwdPredicate pre1 b (fun pre z => ∃ a, p₂ (p₁ pre a) z) :=
+    fun m f => match m with 
+               | MonadFwdPredicate.mk z1 pf1 =>
+                   match (f z1.output) with
+                   | MonadFwdPredicate.mk z2 pf2 =>
+                       MonadFwdPredicate.mk z2 (fun pre => Exists.intro z1.output (pf2 (pf1 pre)))
+
+
+def runFP {α : Type} {pre1 :Prop} {a : α} {p₁ : fPred α} (m : MonadFwdPredicate pre1 a p₁) : pre1 → p₁ pre1 a :=
+  fun p1 => match m with 
+            | MonadFwdPredicate.mk ma pf => pf p1
+
+def sampleProg := runFP (bindFP (retFP 3) (fun _ => bindFP (retFP 5) (fun _ => retFP 4))) (rfl : 2=2)
+
+-- backward transforming predicate
+
+def bPred (α : Type) : Type := (α → Prop) → Prop
+
+-- for backward transformers we need to map pointwise under the transformer. This also restricts transformers to be monotonic
+class MonoBackward (w : bPred α) where
+  monoMap {p₁ p₂ : α → Prop} : (∀ a , p₁ a → p₂ a) → w p₁ → w p₂
+
+def simpleBP {α : Type} (v : α) : bPred α := fun (post : α → Prop) => post v
+
+instance {α : Type} {v : α}: MonoBackward (simpleBP v) where
+  monoMap  {p₁ p₂ : α → Prop} :=  fun f wp1 => f v wp1
+
+inductive MonadBwdPredicate {α : Type} : α → bPred α → (α → Prop) → Type where
+| mk : (mz : BaseMonad α) → (pf : ∀ x, x = mz.output → p post) → MonadBwdPredicate (mz.output) p post
 
 
 
-structure DijkstraMonad {p₁ p₂ : Prop} (α : Type) (z : (α → p₁) → p₂) where
-  (output : α)
+def retBP {α : Type} (v : α) {post : α → Prop} (postpf: post v) : MonadBwdPredicate v (@simpleBP α v) post:=
+  let bm := BaseMonad.mk v
+  MonadBwdPredicate.mk bm (fun x (he : x = bm.output) => postpf)
 
-def DMonad {α : Type} {p₁ p₂ : Prop} (x : α) (wp : (α → p₁) → p₂) := ∀ (p : α → p₁), p₂ → p₁
+def bindBP {α : Type} {a b : α} {post1 : α → Prop} {p₁ p₂ : bPred α} [MonoBackward p₁] :
+  MonadBwdPredicate a p₁ (fun x => ∀ post2, x = a → post2) → (α → MonadBwdPredicate b p₂ post1) → MonadBwdPredicate b (fun post => p₁ (fun x => b = x → p₂ post)) post1 :=
+    fun m f => match m with
+               | MonadBwdPredicate.mk z1 pf1 =>
+                 match (f z1.output) with
+                 | MonadBwdPredicate.mk z2 pf2 =>
+                     MonadBwdPredicate.mk z2 (fun x he =>
+                                                    let (hp : ∃ x, x = z1.output) := Exists.intro z1.output (show _ by rfl)
+                                                    let hx : p₁ fun x => ∀ post2 , x = z1.output → post2 := Exists.elim hp pf1
+                                                    let tx :  ∀ (a : α), (∀ (postx : Prop), a = z1.output → postx) → z2.output = a → p₂ post1 :=
+                                                      fun a postx eq =>
+                                                        let eq' := show _ from Eq.symm eq
+                                                        pf2 a eq'
+                                                    MonoBackward.monoMap tx hx
+                     )
 
-def DMret {α : Type} {p₁ p₂ : Prop} (x : α) { wp : (α → p₁) → p₁} : DMonad x wp :=
-  fun p p2 => p x
+def runBP {α : Type} {post1 : α → Prop} {a : α} {p₁ : bPred α} (m : MonadBwdPredicate a p₁ post1) : ∀ x, x = a → p₁ post1 :=
+  fun a => match m with
+           | MonadBwdPredicate.mk ma pf => pf a
 
-def DMrun {α : Type} {p₁ p₂ : Prop} {x : α} {wp : (α → p₁) → p₂} (d : DMonad x wp) (post : α → p₁) : p₂ := wp post
+#check retBP 3 rfl
 
-#check DMret 2
-#reduce DMrun (DMret 2) (fun a => show ∀ a, a = 2 → true by simp)
-
-def apple {α : Type} {p₁ :Prop} (x : α) (z : α → p₁) : p₁ := z x
-
-def lit (x : Nat) : ∃ b, b = x :=
-  Exists.intro x rfl
-
-def lit2 {p₁ : Prop} {x : α → Prop} (z : ∀ a, x a → p₁) (b : Exists x) : p₁ := Exists.elim b z
-
-def lit3 {p₁ : Prop} (x : α → Prop) (hp : p₁): ∀ a, x a → p₁ :=
-  fun (a : α) _ => show p₁ from hp
-
-def lit4 (a : α) (x : α → Prop) {hp : x a} : Exists x := Exists.intro a hp
-
-def DJRet {α : Type} {p₁ : Prop} {z : (α → p₁) → p₁} (x: α) : DijkstraMonad α := DijkstraMonad.mk x
-
-def DJBind {α β : Type} {p₁ p₂ p₃ : Prop} {wp1 : (α → p₂) → p₃} {wp2 : α → (β → p₁) → p₂} :
-  DijkstraMonad α wp1 → ( (x:α) → DijkstraMonad β (wp2 x)) → DijkstraMonad β (fun p => wp1 (fun x => wp2 x p)) :=
-    fun m1 m2 => let a := DijkstraMonad.output m1
-                 let b := DijkstraMonad.output (m2 a)
-                 DijkstraMonad.mk b
-
-def DJRun {α : Type} {p₁ p₂ :Prop} {wp : (α → p₁) → p₂} (d : DijkstraMonad α wp) (post : α → p₁) : p₂ := wp post
-
-example : ∃ x : Nat, x = 3 :=
-  have h : 3=3 := by rfl
-  Exists.intro 3 h
-
-example (h₁ : ∃ x : Nat, x = 3) (z : ∀ x, x = 3 → a > 1) : a > 1 :=
-  Exists.elim h₁ z
-
-#check (@DJRun Nat (1=1) (1=1) (fun hp => show 1=1 by rfl) (@DJRet Nat (1=1) (fun hp => hp 2) 2) (fun a => show 1=1 by rfl))
-#check @DJRet Nat (1=1) (fun hp => hp 2) 2
-#reduce DJRun (DJRet 2) (fun a => show 1=1 by rfl)
-#check (lit 3)
-#check ∃ x, x = 3
-#check ∀ (a : Nat), a = 3 → true
-#check @Exists
-#check lit2 (lit3 (fun a => a < 3) (show 3=3 by rfl)) (Exists.intro 2 (show (fun a => a < 3) 2 by simp))
-#check lit4 (fun a => a < 3) 2
-#check ∃ a, a < 3
+def sampleBack := runBP (retBP 3 rfl) 3
